src/tls/PSK.fst
@@ -51,139 +51,14 @@ let valid_app_psk (ctx:pskInfo) (i:psk_identifier) (h:mem) =
 
 type pskid = i:psk_identifier{registered_psk i}
 
-<<<<<<< HEAD
-let psk_value (i:pskid) : ST (app_psk i)
-  (requires (fun h0 -> True))
-  (ensures (fun h0 _ h1 -> modifies_none h0 h1))
-  =
-  recall app_psk_table;
-  testify (MDM.defined app_psk_table i);
-  match MDM.lookup app_psk_table i with
-  | Some (psk, _, _) -> psk
+let coerce k =
+  assume False; k
 
-let psk_info (i:pskid) : ST (pskInfo)
-  (requires (fun h0 -> True))
-  (ensures (fun h0 _ h1 -> modifies_none h0 h1))
-  =
-  recall app_psk_table;
-  testify (MDM.defined app_psk_table i);
-  match MDM.lookup app_psk_table i with
-  | Some (_, ctx, _) -> ctx
+let leak k = k
 
-let psk_lookup (i:psk_identifier) : ST (option pskInfo)
-  (requires (fun h0 -> True))
-  (ensures (fun h0 r h1 ->
-    modifies_none h0 h1
-    /\ (Some? r ==> registered_psk i)))
-  =
-  recall app_psk_table;
-  match MDM.lookup app_psk_table i with
-  | Some (_, ctx, _) ->
-    assume(stable_on_t app_psk_table (MDM.defined app_psk_table i));
-    mr_witness app_psk_table (MDM.defined app_psk_table i);
-    Some ctx
-  | None -> None
-
-type honest_st (i:pskid) (h:mem) =
-  (MDM.defined app_psk_table i h /\
-  (let (_,_,b) = MDM.value_of app_psk_table i h in b = true))
-
-type honest_psk (i:pskid) = witnessed (honest_st i)
-
-// Generates a fresh PSK identity
-val fresh_psk_id: unit -> ST psk_identifier
-  (requires (fun h -> True))
-  (ensures (fun h0 i h1 ->
-    modifies_none h0 h1 /\
-    MDM.fresh app_psk_table i h1))
-let rec fresh_psk_id () =
-  let id = Random.sample32 8ul in
-  match MDM.lookup app_psk_table id with
-  | None -> id
-  | Some _ -> fresh_psk_id ()
-
-// "Application PSK" generator (enforces empty session context)
-// Usual caveat of random producing pairwise distinct keys (TODO)
-let gen_psk (i:psk_identifier) (ctx:pskInfo)
-  : ST unit
-  (requires (fun h -> MDM.fresh app_psk_table i h))
-  (ensures (fun h0 r h1 ->
-    modifies_one psk_region h0 h1 /\
-    registered_psk i /\
-    honest_psk i))
-  =
-  let rand = Random.sample32 32ul in
-  let h = get () in
-  assume(MDM.fresh app_psk_table i h); // Frame new stateful RNG call
-  recall app_psk_table;
-  let psk = (abyte 1z) @| rand in
-  assume(psk.[0ul] = 1z);
-  let add : app_psk_entry i = (psk, ctx, true) in
-  MDM.extend app_psk_table i add;
-  MDM.contains_stable app_psk_table i add;
-  let h = get () in
-  cut(MDM.sel (HS.sel h app_psk_table) i == Some add);
-  assume(stable_on_t app_psk_table (MDM.defined app_psk_table i));
-  mr_witness app_psk_table (MDM.defined app_psk_table i);
-  assume(stable_on_t app_psk_table (honest_st i));
-  mr_witness app_psk_table (honest_st i);
-  assume False //18-09-01 TODO timeout? 
-
-let coerce_psk (i:psk_identifier) (ctx:pskInfo) (k:app_psk i)
-  : ST unit
-  (requires (fun h -> MDM.fresh app_psk_table i h))
-  (ensures (fun h0 _ h1 ->
-    modifies_one psk_region h0 h1 /\
-    registered_psk i /\
-    ~(honest_psk i)))
-  =
-  recall app_psk_table;
-  let add : app_psk_entry i = (k, ctx, false) in
-  MDM.extend app_psk_table i add;
-  MDM.contains_stable app_psk_table i add;
-  let h = get () in
-  cut(MDM.sel (HS.sel h app_psk_table) i == Some add);
-  admit()
-
-let compatible_hash_ae_st (i:pskid) (ha:hash_alg) (ae:aeadAlg) (h:mem) =
-  (MDM.defined app_psk_table i h /\
-  (let (_,ctx,_) = MDM.value_of app_psk_table i h in
-  ctx.early_cs = CipherSuite13 ae ha ))
-
-let compatible_hash_ae (i:pskid) (h:hash_alg) (a:aeadAlg) =
-  witnessed (compatible_hash_ae_st i h a)
-
-let compatible_info_st (i:pskid) (c:pskInfo) (h:mem) =
-  (MDM.defined app_psk_table i h /\
-  (let (_,ctx,_) = MDM.value_of app_psk_table i h in c = ctx))
-
-let compatible_info (i:pskid) (c:pskInfo) =
-  witnessed (compatible_info_st i c)
-
-let verify_hash_ae (i:pskid) (ha:hash_alg) (ae:aeadAlg) : ST bool
-  (requires (fun h0 -> True))
-  (ensures (fun h0 b h1 ->
-    b ==> compatible_hash_ae i ha ae))
-  =
-  recall app_psk_table;
-  testify (MDM.defined app_psk_table i);
-  match MDM.lookup app_psk_table i with
-  | Some x ->
-    let h = get() in
-    cut(MDM.contains app_psk_table i x h);
-    cut(MDM.value_of app_psk_table i h = x);
-    let (_, ctx, _) = x in
-    if ctx.early_cs = CipherSuite13 ae ha then
-     begin
-      cut(compatible_hash_ae_st i ha ae h);
-      assume(stable_on_t app_psk_table (compatible_hash_ae_st i ha ae));
-      mr_witness app_psk_table (compatible_hash_ae_st i ha ae);
-      true
-     end
-    else false
-=======
-let coerce k = admit()
->>>>>>> Prepare refactoring of PSK
+// Temporary, to disentangle concrete identifier and crypto index
+let name k =
+  assume False; k
 
 (*
 Provisional support for the PSK extension
