src/tls/Ticket.fst
@@ -41,7 +41,7 @@ private let dummy_id (a:aeadAlg) : St AE.id =
   let h = Hashing.Spec.SHA2_256 in
   let li = LogInfo_CH0 ({
     li_ch0_cr = Bytes.create 32ul 0z;
-    li_ch0_ed_psk = empty_bytes;
+    li_ch0_ed_psk = PSK.coerce empty_bytes;
     li_ch0_ed_ae = a;
     li_ch0_ed_hash = h;
   }) in
